Wrong fix for einst

theories/Inst.v
@@ -5,9 +5,21 @@ From LocalComp.autosubst Require Import AST SubstNotations RAsimpl AST_rasimpl.
 From LocalComp Require Import Util BasicAST Env.
 Import ListNotations.
 
+(**
+
+  The argument [t] of [einst ξ t] is expected to be closed.
+  This is the reason why we use a dummy value for variables, this way we don't
+  need to worry about the function being partial.
+  Thanks to this, we also don't need to worry about lifting [ξ] when going under
+  binders.
+
+**)
+
+Definition dummy := Sort 0.
+
 Fixpoint einst (ξ : eargs) (t : term) :=
   match t with
-  | var n => var n
+  | var n => dummy
   | Sort i => Sort i
   | Pi A B => Pi (einst ξ A) (einst ξ B)
   | lam A t => lam (einst ξ A) (einst ξ t)
