theories/BasicMetaTheory.v
@@ -110,16 +110,13 @@ Qed.
 
 Lemma ren_inst :
   ∀ ρ ξ t,
-    ρ ⋅ (einst ξ t) = einst (map (map (ren_term ρ)) ξ) (ρ ⋅ t).
+    ρ ⋅ (einst ξ t) = einst (map (map (ren_term ρ)) ξ) t.
 Proof.
   intros ρ ξ t.
   induction t in ρ |- *. all: try solve [ eauto ].
   - cbn. f_equal. 1: eauto.
     rewrite IHt2. f_equal.
-    (* This is wrong, need to figure out who lives where.
-      It seems it doesn't make sense for an argument to einst to feature
-      free variables.
-    *)
+    (* Still wrong? *)
 Abort.
 
 Lemma conv_ren :
